A_setup.v
@@ -4,6 +4,8 @@ Require Vector.
 Require Import Utf8 Bool List PeanoNat PArith BinNums.
 Export Utf8 List ListNotations PeanoNat PArith BinNums.
 
+Open Scope positive.
+
 (******************************************************************************)
 (* I. Global notations.                                                       *)
 (******************************************************************************)
