C1_Schreier_vector.v
@@ -1,6 +1,6 @@
 (* A functional Schreier-vector to compute orbits. *)
 
-From permutation_solver Require Import A_setup B1_finite_map B2_permutation.
+From Permutations Require Import A_setup B1_finite_map B2_permutation.
 
 Module Schreier.
 
